src/ValueFlagComp.v
@@ -593,6 +593,7 @@ Lemma compile_not_value : forall a b,
 induction a using A.expr_ind'; intros0 Hcomp; simpl in *; refold_compile; subst; inversion 1.
 Qed.
 
+
 Lemma compile_cases_arent_values : forall a b,
     compile a = b ->
     B.cases_arent_values b.
@@ -609,6 +610,22 @@ simpl; B.refold_cases_arent_values; eauto.
   rewrite <- Forall_map.
   list_magic_on (cases, tt). eauto using compile_not_value.
 Qed.
+
+Lemma compile_list_cases_arent_values : forall a b,
+    compile_list a = b ->
+    Forall B.cases_arent_values b.
+induction a;
+intros0 Hcomp; simpl in *; refold_compile; subst; eauto using compile_cases_arent_values.
+Qed.
+
+Theorem compile_cu_cases_arent_values : forall a ameta b bmeta,
+    compile_cu (a, ameta) = (b, bmeta) ->
+    Forall B.cases_arent_values b.
+intros.
+simpl in *. inject_pair.
+eauto using compile_list_cases_arent_values.
+Qed.
+
 
 Lemma compile_no_values : forall a b,
     compile a = b ->
@@ -894,6 +911,29 @@ all: simpl in *; B.refold_cases_arent_values; repeat break_and.
 Qed.
 
 
+Inductive I' : A.state -> B.state -> Prop :=
+| I'_intro : forall a b,
+        I a b ->
+        B.state_cases_arent_values b ->
+        I' a b.
+
+Theorem I'_sim : forall AE BE a a' b,
+    compile_list AE = BE ->
+    Forall B.cases_arent_values BE ->
+    I' a b ->
+    A.sstep AE a a' ->
+    exists b',
+        B.splus BE b b' /\
+        I' a' b'.
+intros. on >I', invc.
+fwd eapply I_sim; eauto.
+  { on >B.state_cases_arent_values, invc; simpl; auto. }
+break_exists; break_and.
+eexists; split; eauto. constructor; eauto.
+eapply B.state_cases_arent_values_inductive_plus; eassumption.
+Qed.
+
+
 
 Require Semantics.
 
@@ -904,26 +944,17 @@ Section Preservation.
 
   Hypothesis TRANSF : compile_cu prog = tprog.
 
-  
-  (* Inductive match_states (AE : A.env) (BE : B.env) : A.expr -> B.expr -> Prop := *)
-  (* | match_st : *)
-  (*     forall a b, *)
-  (*       R AE BE a b -> *)
-  (*       match_states AE BE a b. *)
-
-  (* Lemma step_sim : *)
-  (*   forall AE BE a b, *)
-  (*     match_states AE BE a b -> *)
-  (*     forall a', *)
-  (*       A.step AE a a' -> *)
-  (*       exists b', *)
-  (*         splus (B.step BE) b b'. *)
-  (* Proof. *)
-  (* Admitted. *)
-
   Theorem fsim :
     Semantics.forward_simulation (A.semantics prog) (B.semantics tprog).
   Proof.
-  Admitted.
+    eapply Semantics.forward_simulation_plus with (match_states := I').
+    - inversion 1. (* TODO - replace with callstate matching *)
+    - intros0 II Afinal. invc Afinal. invc II. on >I, invc. constructor.
+    - intros0 Astep. intros0 II.
+      eapply splus_semantics_sim, I'_sim; eauto.
+      + destruct prog, tprog. unfold compile_cu in *. inject_pair. auto.
+      + destruct prog, tprog. unfold compile_cu in *. inject_pair.
+        simpl. eauto using compile_list_cases_arent_values.
+  Qed.
 
 End Preservation.
